modeled preprocess

SHA256/Preprocess.v
@@ -23,29 +23,63 @@ Require Import Eager.
 Require Import Prims.
 Require Import SHA256.
 
-(* TODO *)
-Definition preprocess_spec (msg : ext_val) : ext_val := eseq nil.
+Definition preprocess_spec (padding msglen : Z) (msg : ext_val) : ext_val :=
+  match msg with
+  | eseq l => 
+    (split_ev (Z.to_nat 512)
+            (eseq
+               (l ++
+                  [ebit true] ++
+                  repeat (ebit false) (Z.to_nat padding) ++
+                  @ExtToBitvector.from_bitv (Z.to_nat 64) (repr msglen))))
+  | _ => eseq nil
+  end.
 
+Lemma from_bitv_ext_type :
+  forall y x (bv : BitV x),
+    Forall (fun x => has_type x tbit) (ExtToBitvector.from_bitv' x y bv).
+Proof.
+  induction y; intros.
+  simpl.
+  econstructor.
+  simpl.
+  econstructor.
+  econstructor.
+  eauto.
+Qed.
+
+Lemma strictval_from_bitv_ext :
+  forall y x (bv : BitV x),
+    strictval_from_bitv' x y bv = map to_sval (ExtToBitvector.from_bitv' x y bv).
+Proof.
+  induction y; intros;
+    simpl. reflexivity.
+  f_equal.
+  eauto.
+Qed.
 
 Lemma preprocess_eval :
   forall msg len,
     has_type msg (tseq len tbit) ->
     forall GE TE SE,
       wf_env ge GE TE SE ->
-      forall ta1 ta2 ta3 ta4 tv1 tv2 tv3 padding emsg,
-        eager_eval_type GE TE ta1 tv1 ->
-        eager_eval_type GE TE ta2 tv2 ->
-        eager_eval_type GE TE ta3 tv3 ->
+      forall ta1 ta2 ta3 ta4 msglen contentlen chunks padding emsg,
+        eager_eval_type GE TE ta1 (tvnum msglen) ->
+        eager_eval_type GE TE ta2 (tvnum contentlen) ->
+        eager_eval_type GE TE ta3 (tvnum chunks) ->
         eager_eval_type GE TE ta4 (tvnum padding) ->
         eager_eval_expr GE TE SE emsg (to_sval msg) ->
         forall res,
-          res = to_sval (preprocess_spec msg) ->
+          res = to_sval (preprocess_spec padding msglen msg) ->
           eager_eval_expr GE TE SE (EApp (ETApp (ETApp (ETApp (ETApp (EVar preprocess) (ETyp ta1)) (ETyp ta2)) (ETyp ta3)) (ETyp ta4)) emsg) res.
 Proof.
   intros.
   gen_global preprocess.
   gen_global (37,"split").
   gen_global (34,"#").
+  gen_global (29,"zero").
+  gen_global (0,"demote").
+  gen_global (9,"True").
   inversion H. subst len msg t.
   e. e. e. e. e. ag.
   e. e. e. e. 
@@ -59,15 +93,43 @@ Proof.
   simpl.
   instantiate (1 := (ebit true) :: nil).
   simpl. e.
-  gen_global (9,"True").
   ag.
   e. reflexivity. reflexivity.
 
   use append_eval; try lv.
+  use zero_eval; try lv.
+
+  simpl. reflexivity.
+  use demote_eval; try lv.
+  simpl. unfold strictnum.
+  f_equal. f_equal.
+
+  instantiate (1 := ExtToBitvector.from_bitv (repr msglen)).
+  unfold strictval_from_bitv.
+  unfold ExtToBitvector.from_bitv.
+  instantiate (1 := Z.to_nat 64).
+
+  eapply strictval_from_bitv_ext.
+
+  reflexivity.
+  reflexivity.
+  reflexivity.
+  econstructor.
+  eapply Forall_app; split.
+  inversion H. eauto.
+  eapply Forall_app; split.
+  repeat econstructor.
+  eapply Forall_app; split.
+  eapply repeat_Forall. econstructor.
+
+
+  eapply from_bitv_ext_type; eauto.
+
+  subst res.
+  unfold ExtToBitvector.from_bitv.
+  reflexivity.
   
-  
-  
-Admitted.  
+Qed.
 
 
     
